Done some sbt tasks

inference-tool/src/main/scala/inference/Dirties.scala
@@ -120,16 +120,16 @@ object Dirties {
 
   def initiallyUndefinedContextCheck(e: iEFSM, r: Nat.nat, s: Nat.nat): Boolean = {
     // TODO: Fix the exception thrown here
-    val f = "intermediate_"+System.currentTimeMillis()
-    TypeConversion.efsmToSALTranslator(Inference.tm(e), f)
-
-    addLTL("salfiles/" + f + ".sal", s"  initiallyUndefined: THEOREM MichaelsEFSM |- G(cfstate = State_${valueOf(s)} => r_${valueOf(r)} = ValueOption ! None);")
-
-    val output = Seq("bash", "-c", "cd salfiles; sal-smc --assertion='" + f + "{100}!initiallyUndefined'").!!
-    if (output.toString != "proved.\n") {
-      print(output)
-    }
-    return (output.toString == "proved.\n")
+    // val f = "intermediate_"+System.currentTimeMillis()
+    // TypeConversion.efsmToSALTranslator(Inference.tm(e), f)
+    //
+    // addLTL("salfiles/" + f + ".sal", s"  initiallyUndefined: THEOREM MichaelsEFSM |- G(cfstate = State_${valueOf(s)} => r_${valueOf(r)} = value_option ! None);")
+    //
+    // val output = Seq("bash", "-c", "cd salfiles; sal-smc --assertion='" + f + "{100}!initiallyUndefined'").!!
+    // if (output.toString != "proved.\n") {
+    //   print(output)
+    // }
+    // return (output.toString == "proved.\n")
     return true
   }
 
@@ -138,32 +138,31 @@ object Dirties {
     case Value.Numa(n) => s"NUM(${valueOf(n)})"
   }
 
-
   def generaliseOutputContextCheck(l: String, ePrime: iEFSM, e: iEFSM, r: Nat.nat, v: Value.value, s_old: Nat.nat, s_new: Nat.nat): Boolean = {
-    val f_old = "orig_"+System.currentTimeMillis()
-    TypeConversion.efsmToSALTranslator(Inference.tm(e), f_old)
-    val inxLabel = Code_Generation.input_updates_register(ePrime)
-    addLTL("salfiles/" + f_old + s".sal", s"  inputValue: THEOREM MichaelsEFSM |-\n" +
-      s"    U(cfstate /= NULL_STATE, cfstate=State_${valueOf(s_old)}) =>\n"+
-      s"    U(label = ${inxLabel._2} => I(1) = ${salValue(v)}, X(cfstate = NULL_STATE));")
-
-    val f_new = "intermediate_"+System.currentTimeMillis()
-    TypeConversion.efsmToSALTranslator(Inference.tm(ePrime), f_new)
-    addLTL("salfiles/" + f_new + ".sal", s"  generaliseOutput: THEOREM MichaelsEFSM |-\n"+
-      s"    U(cfstate /= NULL_STATE, cfstate = State_${valueOf(s_new)}) =>\n"+
-      s"    U(label = select => I(${valueOf(inxLabel._1)}) = ${salValue(v)}, cfstate = NULL_STATE) =>\n"+
-      s"    U(cfstate = State_${valueOf(s_new)} => r_1 = Some(${salValue(v)}), cfstate=NULL_STATE);")
-
-
-    println(s"sal-smc --assertion='${f_old}{100}!inputValue'")
-    val output1 = Seq("bash", "-c", s"cd salfiles; sal-smc --assertion='${f_old}{100}!inputValue'").!!
-    println(output1)
-
-    println(s"sal-smc --assertion='${f_new}{100}!generaliseOutput'")
-    val output2 = Seq("bash", "-c", s"cd salfiles; sal-smc --assertion='${f_new}{100}!generaliseOutput'").!!
-    println(output2)
-
-    return (output1.toString == "proved.\n" && output2.toString == "proved.\n")
+    // val f_old = "orig_"+System.currentTimeMillis()
+    // TypeConversion.efsmToSALTranslator(Inference.tm(e), f_old)
+    // val inxLabel = Code_Generation.input_updates_register(ePrime)
+    // addLTL("salfiles/" + f_old + s".sal", s"  inputValue: THEOREM MichaelsEFSM |-\n" +
+    //   s"    U(cfstate /= NULL_STATE, cfstate=State_${valueOf(s_old)}) =>\n"+
+    //   s"    U(label = ${inxLabel._2} => I(1) = ${salValue(v)}, X(cfstate = NULL_STATE));")
+    //
+    // val f_new = "intermediate_"+System.currentTimeMillis()
+    // TypeConversion.efsmToSALTranslator(Inference.tm(ePrime), f_new)
+    // addLTL("salfiles/" + f_new + ".sal", s"  generaliseOutput: THEOREM MichaelsEFSM |-\n"+
+    //   s"    U(cfstate /= NULL_STATE, cfstate = State_${valueOf(s_new)}) =>\n"+
+    //   s"    U(label = select => I(${valueOf(inxLabel._1)}) = ${salValue(v)}, cfstate = NULL_STATE) =>\n"+
+    //   s"    U(cfstate = State_${valueOf(s_new)} => r_1 = Some(${salValue(v)}), cfstate=NULL_STATE);")
+    //
+    //
+    // println(s"sal-smc --assertion='${f_old}{100}!inputValue'")
+    // val output1 = Seq("bash", "-c", s"cd salfiles; sal-smc --assertion='${f_old}{100}!inputValue'").!!
+    // println(output1)
+    //
+    // println(s"sal-smc --assertion='${f_new}{100}!generaliseOutput'")
+    // val output2 = Seq("bash", "-c", s"cd salfiles; sal-smc --assertion='${f_new}{100}!generaliseOutput'").!!
+    // println(output2)
+    //
+    // return (output1.toString == "proved.\n" && output2.toString == "proved.\n")
     return true
   }
 
@@ -173,25 +172,9 @@ object Dirties {
                             s_prime: Nat.nat,
                             t1: Transition.transition_ext[Unit],
                             t2: Transition.transition_ext[Unit]): Boolean = {
-                              if (HOL.equal(t1, t2)) {
-                                return true
-                              }
-                              // println(f"\nDoes ${PrettyPrinter.transitionToString(t1)} directly subsume ${PrettyPrinter.transitionToString(t2)}? y/n")
-                              if (Code_Generation.always_different_outputs(Transition.Outputs(t1), Transition.Outputs(t2))) {
+                              if (Store_Reuse_Subsumption.drop_guard_add_update_direct_subsumption(t2, t1, b, s_prime)) {
                                 // println("n")
                                 return false
-                              }
-                              else if (Store_Reuse_Subsumption.drop_guard_add_update_direct_subsumption(t1, t2, b, s_prime)) {
-                                // println("y")
-                                return true
-                              }
-                              else if (Store_Reuse_Subsumption.drop_guard_add_update_direct_subsumption(t2, t1, b, s_prime)) {
-                                // println("n")
-                                return false
-                              }
-                              else if (Store_Reuse_Subsumption.generalise_output_direct_subsumption(t1, t2, b, a, s, s_prime)) {
-                                // println("y")
-                                return true
                               }
                               else if (Store_Reuse_Subsumption.generalise_output_direct_subsumption(t2, t1, b, a, s, s_prime)) {
                                 // println("n")
